\documentclass[../main.tex]{subfiles}
\begin{document}

\chapter{Systems of differential equations}
\label{chap:chap_20}
%\pagenumbering{arabic}

\noindent Many mathematical models involve $m+1$ unknown functions governed by a system of $m+1$ differential equations. In abstract form we may denote the unknowns by $u^{(0)}, \ldots, u^{(m)}$ and write the governing equations as
$$
\begin{gathered}
	\mathcal{L}_{0}\left(u^{(0)}, \ldots, u^{(m)}\right)=0 \\
	\vdots \\
	\mathcal{L}_{m}\left(u^{(0)}, \ldots, u^{(m)}\right)=0
\end{gathered}
$$
where $\mathcal{L}_{i}$ is some differential operator defining differential equation number $i$.\smallbreak
	\section[Systems of differential equations]{Variational forms}
		\label{sec:sec_20_1}
		\noindent There are basically two ways of formulating a variational form for a system of differential equations. The first method treats each equation independently as a scalar equation, while the other method views the total system as a vector equation with a vector function as unknown.
		
		Let us start with the one equation at a time approach. We multiply equation number $i$ by some test function $v^{(i)} \in V^{(i)}$ and integrate over the domain:
		
		\begin{equation}
		\label{eqa256}
			\int_{\Omega} \mathcal{L}^{(0)}\left(u^{(0)}, \ldots, u^{(m)}\right) v^{(0)} \mathrm{d} x=0 \\
		\end{equation}
			
		\begin{equation}
		\label{eqa257}
			\vdots \\
		\end{equation}
	
		\begin{equation}
		\label{eqa258}
			\int_{\Omega} \mathcal{L}^{(m)}\left(u^{(0)}, \ldots, u^{(m)}\right) v^{(m)} \mathrm{d} x=0
		\end{equation}
	
		\noindent Terms with second-order derivatives may be integrated by parts, with Neumann conditions inserted in boundary integrals. Let
		$$
		V^{(i)}=\operatorname{span}\left\{\psi_{0}^{(i)}, \ldots, \psi_{N_{i}}^{(i)}\right\},
		$$
		such that
		$$
		u^{(i)}=B^{(i)}(\boldsymbol{x})+\sum_{j=0}^{N_{i}} c_{j}^{(i)} \psi_{j}^{(i)}(\boldsymbol{x}),
		$$
		where $B^{(i)}$ is a boundary function to handle nonzero Dirichlet conditions. Observe that different unknowns live in different spaces with different basis functions and numbers of degrees of freedom.
		
		From the $m$ equations in the variational forms we can derive $m$ coupled systems of algebraic equations for the $\prod_{i=0}^{m} N_{i}$ unknown coefficients $c_{j}^{(i)}, j=$ $0, \ldots, N_{i}, i=0, \ldots, m$.\smallbreak
		
		The alternative method for deriving a variational form for a system of differential equations introduces a vector of unknown functions
		$$
		\boldsymbol{u}=\left(u^{(0)}, \ldots, u^{(m)}\right)
		$$
		a vector of test functions
		$$
		\boldsymbol{v}=\left(u^{(0)}, \ldots, u^{(m)}\right)
		$$
		with
		$$
		\boldsymbol{u}, \boldsymbol{v} \in \boldsymbol{V}=V^{(0)} \times \cdots \times V^{(m)} .
		$$
		With nonzero Dirichlet conditions, we have a vector $\boldsymbol{B}=\left(B^{(0)}, \ldots, B^{(m)}\right)$ with boundary functions and then it is $u-B$ that lies in $V$, not $u$ itself. \smallbreak
		The governing system of differential equations is written
		$$
		\mathcal{L}(\boldsymbol{u})=0,
		$$
		where
		$$
		\mathcal{L}(\boldsymbol{u})=\left(\mathcal{L}^{(0)}(\boldsymbol{u}), \ldots, \mathcal{L}^{(m)}(\boldsymbol{u})\right)
		$$
		The variational form is derived by taking the inner product of the vector of equations and the test function vector:
		
		\begin{equation}
			\label{eqa259}
			\int_{\Omega} \mathcal{L}(\boldsymbol{u}) \cdot \boldsymbol{v}=0 \quad \forall \boldsymbol{v} \in \boldsymbol{V} .
		\end{equation}
	
		Observe that (\ref{eqa259}) is one scalar equation. To derive systems of algebraic equations for the unknown coefficients in the expansions of the unknown functions, one chooses $m$ linearly independent $\boldsymbol{v}$ vectors to generate $m$ independent variational forms from (\ref{eqa259}). The particular choice $v=\left(v^{(0)}, 0, \ldots, 0\right)$ recovers (\ref{eqa256}), $\boldsymbol{v}=\left(0, \ldots, 0, v^{(m)}\right.$ recovers $(258)$, and $\boldsymbol{v}=\left(0, \ldots, 0, v^{(i)}, 0, \ldots, 0\right)$ recovers the variational form number i, $\int_{\Omega} \mathcal{L}^{(i)} v^{(i)} \mathrm{d} x=0$, in (\ref{eqa256})-(\ref{eqa258}).\bigbreak
	\section[A worked example]{A worked example}
		\label{sec:sec_20_2}
		\noindent We now consider a specific system of two partial differential equations in two space dimensions:
		
		\begin{equation}
			\label{eqa260}
			\mu \nabla^{2} w=-\beta \\
		\end{equation}
	
		\begin{equation}
			\label{eqa261}
			\kappa \nabla^{2} T=-\mu\|\nabla w\|^{2}
		\end{equation}
		
		\noindent The unknown functions $w(x, y)$ and $T(x, y)$ are defined in a domain $\Omega$, while $\mu, \beta$, and $\kappa$ are given constants. The norm in (\ref{eqa261}) is the standard Eucledian norm:
		$$
		\|\nabla w\|^{2}=\nabla w \cdot \nabla w=w_{x}^{2}+w_{y}^{2}
		$$
		The boundary conditions associated with (\ref{eqa260})-(\ref{eqa261}) are $w=0$ on $\partial \Omega$ and $T=T_{0}$ on $\partial \Omega$. Each of the equations (\ref{eqa260}) and (\ref{eqa261}) need one condition at each point on the boundary.
		
		The system (\ref{eqa260})-(\ref{eqa261}) arises from fluid flow in a straight pipe, with the $z$ axis in the direction of the pipe. The domain $\Omega$ is a cross section of the pipe, $w$ is the velocity in the $z$ direction, $\mu$ is the viscosity of the fluid, $\beta$ is the pressure gradient along the pipe, $T$ is the temperature, and $\kappa$ is the heat conduction coefficient of the fluid. The equation $(260)$ comes from the Navier-Stokes equations, and (261) follows from the energy equation. The term $-\mu\|\nabla w\|^{2}$ models heating of the fluid due to internal friction.
		
		Observe that the system (\ref{eqa260})-(\ref{eqa261}) has only a one-way coupling: $T$ depends on $w$, but $w$ does not depend on $T$, because we can solve (\ref{eqa260}) with respect to $w$ and then (\ref{eqa261}) with respect to $T$. Some may argue that this is not a real system of PDEs, but just two scalar PDEs. Nevertheless, the one-way coupling is convenient when comparing different variational forms and different implementations.
	\section[Identical function spaces for the unknowns]{Identical function spaces for the unknowns}
		\label{sec:sec_20_3}
		\noindent Let us first apply the same function space $V$ for $w$ and $T$ (or more precisely, $w \in V$ and $\left.T-T_{0} \in V\right)$. With
		$$
		V=\operatorname{span}\left\{\psi_{0}(x, y), \ldots, \psi_{N}(x, y)\right\}
		$$
		we write
		
		\begin{equation}
			\label{eqa262}
		w=\sum_{j=0}^{N} c_{j}^{(w)} \psi_{j}, \quad T=T_{0}+\sum_{j=0}^{N} c_{j}^{(T)} \psi_{j}
		\end{equation}
	
		\noindent Note that $w$ and $T$ in (\ref{eqa260})-(\ref{eqa261}) denote the exact solution of the PDEs, while $w$ and T (\ref{eqa262}) are the discrete functions that approximate the exact solution. It should be clear from the context whether a symbol means the exact or approximate solution, but when we need both at the same time, we use a subscript e to denote the exact solution.\bigbreak
		
		\noindent \textbf{Variational form of each individual PDE.   } Inserting the expansions (\ref{eqa262}) in the governing PDEs, results in a residual in each equation,
		
		\begin{equation}
			\label{eqa263}
			R_{w}=\mu \nabla^{2} w+\beta \\
		\end{equation}
	
		\begin{equation}
			\label{eqa264}
			R_{T}=\kappa \nabla^{2} T+\mu\|\nabla w\|^{2}
		\end{equation}
		
		\noindent A Galerkin method demands $R_{w}$ and $R_{T}$ do be orthogonal to $V$ :
		$$
		\begin{aligned}
			&\int_{\Omega} R_{w} v \mathrm{~d} x=0 \quad \forall v \in V \\
			&\int_{\Omega} R_{T} v \mathrm{~d} x=0 \quad \forall v \in V
		\end{aligned}
		$$
		Because of the Dirichlet conditions, $v=0$ on $\partial \Omega$. We integrate the Laplace terms by parts and note that the boundary terms vanish since $v=0$ on $\partial \Omega$ :
		
		\begin{equation}
			\label{eqa265}
			\int_{\Omega} \mu \nabla w \cdot \nabla v \mathrm{~d} x=\int_{\Omega} \beta v \mathrm{~d} x \quad \forall v \in V \\
		\end{equation}
	
		\begin{equation}
			\label{eqa266}
			\int_{\Omega} \kappa \nabla T \cdot \nabla v \mathrm{~d} x=\int_{\Omega} \mu \nabla w \cdot \nabla w v \mathrm{~d} x \quad \forall v \in V
		\end{equation}
		
		\noindent \textbf{Compound scalar variational form.   } The alternative way of deriving the variational from is to introduce a test vector function $v \in V=V \times V$ and take the inner product of $v$ and the residuals, integrated over the domain:
		$$
		\int_{\Omega}\left(R_{w}, R_{T}\right) \cdot \boldsymbol{v} \mathrm{d} x=0 \quad \forall \boldsymbol{v} \in \boldsymbol{V}
		$$
		With $\boldsymbol{v}=\left(v_{0}, v_{1}\right)$ we get
		$$
		\int_{\Omega}\left(R_{w} v_{0}+R_{T} v_{1}\right) \mathrm{d} x=0 \quad \forall v \in \boldsymbol{V} .
		$$
		Integrating the Laplace terms by parts results in
		
		\begin{equation}
			\label{eqa267}
			\int_{\Omega}\left(\mu \nabla w \cdot \nabla v_{0}+\kappa \nabla T \cdot \nabla v_{1}\right) \mathrm{d} x=\int_{\Omega}\left(\beta v_{0}+\mu \nabla w \cdot \nabla w v_{1}\right) \mathrm{d} x, \quad \forall v \in \boldsymbol{V} . \text { (267) }
		\end{equation}
	
		\noindent Choosing $v_{0}=v$ and $v_{1}=0$ gives the variational form (\ref{eqa265}), while $v_{0}=0$ and $v_{1}=v$ gives (\ref{eqa266})\smallbreak
		With the inner product notation, $(p, q)=\int_{\Omega} p q \mathrm{~d} x$, we can alternatively write (\ref{eqa265}) and (\ref{eqa266}) as
		$$
		\begin{aligned}
			&(\mu \nabla w, \nabla v)=(\beta, v) \quad \forall v \in V \\
			&(\kappa \nabla T, \nabla v)=(\mu \nabla w, \nabla w, v) \quad \forall v \in V
		\end{aligned}
		$$
		or since $\mu$ and $\kappa$ are considered constant,
		
		\begin{equation}
			\label{eqa268}
			\mu(\nabla w, \nabla v)=(\beta, v) \quad \forall v \in V \\
		\end{equation}
	
		\begin{equation}
		\label{eqa269}
			\kappa(\nabla T, \nabla v)=\mu(\nabla w \cdot \nabla w, v) \quad \forall v \in V
		\end{equation}
		
		\noindent \textbf{Decoupled linear systems.   } The linear systems governing the coefficients $c_{j}^{(w)}$ and $c_{j}^{(T)}, j=0, \ldots, N$, are derived by inserting the expansions (\ref{eqa262}) in (\ref{eqa265}) and (\ref{eqa266}), and choosing $v=\psi_{i}$ for $i=0, \ldots, N$. The result becomes
	
		\begin{equation}
			\label{eqa270}
			\sum_{j=0}^{N} A_{i, j}^{(w)} c_{j}^{(w)}=b_{i}^{(w)}, \quad i=0, \ldots, N, \\
		\end{equation}
	
		\begin{equation}
			\label{eqa271}
			\sum_{j=0}^{N} A_{i, j}^{(T)} c_{j}^{(T)}=b_{i}^{(T)}, \quad i=0, \ldots, N, \\
		\end{equation}
	
		\begin{equation}
			\label{eqa272}
			A_{i, j}^{(w)} =\mu\left(\nabla \psi_{j}, \nabla \psi_{i}\right) \\
		\end{equation}
	
		\begin{equation}
			\label{eqa273}
			b_{i}^{(w)} =\left(\beta, \psi_{i}\right), \\
		\end{equation}
	
		\begin{equation}
			\label{eqa274}
			A_{i, j}^{(T)} =\kappa\left(\nabla \psi_{j}, \nabla \psi_{i}\right), \\
		\end{equation}
	
		\begin{equation}
			\label{eqa275}
			b_{i}^{(T)} =\mu\left(\left(\sum_{j} c_{j}^{(w)} \nabla \psi_{j}\right) \cdot\left(\sum_{k} c_{k}^{(w)} \nabla \psi_{k}\right), \psi_{i}\right) .
		\end{equation}
	
		It can also be instructive to write the linear systems using matrices and vectors. Define $K$ as the matrix corresponding to the Laplace operator $\nabla^{2}$. That is, $K_{i, j}=\left(\nabla \psi_{j}, \nabla \psi_{i}\right)$. Let us introduce the vectors
		$$
		\begin{aligned}
			b^{(w)} &=\left(b_{0}^{(w)}, \ldots, b_{N}^{(w)}\right) \\
			b^{(T)} &=\left(b_{0}^{(T)}, \ldots, b_{N}^{(T)}\right) \\
			c^{(w)} &=\left(c_{0}^{(w)}, \ldots, c_{N}^{(w)}\right) \\
			c^{(T)} &=\left(c_{0}^{(T)}, \ldots, c_{N}^{(T)}\right)
		\end{aligned}
		$$
		The system (\ref{eqa270})-(\ref{eqa271}) can now be expressed in matrix-vector form as
		
		\begin{equation}
			\label{eqa276}
			\mu K c^{(w)}=b^{(w)} \\
		\end{equation}
	
		\begin{equation}
			\label{eqa277}
			\kappa K c^{(T)}=b^{(T)}
		\end{equation}
		
		We can solve the first system for $c^{(w)}$, and then the right-hand side $b^{(T)}$ is known such that we can solve the second system for $c^{(T)}$.\bigbreak
		
		\noindent \textbf{Coupled linear systems.   } Despite the fact that $w$ can be computed first, without knowing $T$, we shall now pretend that $w$ and $T$ enter a two-way coupling such that we need to derive the algebraic equations as one system for all the unknowns $c_{j}^{(w)}$ and $c_{j}^{(T)}, j=0, \ldots, N$. This system is nonlinear in $c_{j}^{(w)}$ because of the $\nabla w \cdot \nabla w$ product. To remove this nonlinearity, imagine that we introduce an iteration method where we replace $\nabla w \cdot \nabla w$ by $\nabla w_{-} \cdot \nabla w$, weing the $w$ computed in the previous iteration. Then the term $\nabla w_{-} \cdot \nabla w$ is linear in $w$ since $w_{-}$is known. The total linear system becomes
		
		\begin{equation}
			\label{eqa278}
			\sum_{j=0}^{N} A_{i, j}^{(w, w)} c_{j}^{(w)}+\sum_{j=0}^{N} A_{i, j}^{(w, T)} c_{j}^{(T)} =b_{i}^{(w)}, \quad i=0, \ldots, N, \\
		\end{equation}
	
		\begin{equation}
			\label{eqa279}
			\sum_{j=0}^{N} A_{i, j}^{(T, w)} c_{j}^{(w)}+\sum_{j=0}^{N} A_{i, j}^{(T, T)} c_{j}^{(T)} =b_{i}^{(T)}, \quad i=0, \ldots, N, \\
		\end{equation}
	
		\begin{equation}
			\label{eqa280}
			A_{i, j}^{(w, w)} =\mu\left(\nabla \psi_{j}, \psi_{i}\right), \\
		\end{equation}
	
		\begin{equation}
			\label{eqa281}
			A_{i, j}^{(w, T)} =0, \\
		\end{equation}
	
		\begin{equation}
			\label{eqa282}
			b_{i}^{(w)} =\left(\beta, \psi_{i}\right), \\
		\end{equation}

		\begin{equation}
			\label{eqa283}	
			A_{i, j}^{(w, T)} \left.=\mu\left(\left(\nabla \psi_{-}\right) \cdot \nabla \psi_{j}\right), \psi_{i}\right), \\
		\end{equation}
	
		\begin{equation}
			\label{eqa284}
			A_{i, j}^{(T, T)}=\kappa\left(\nabla \psi_{j}, \psi_{i}\right), \\
		\end{equation}
	
		\begin{equation}
			\label{eqa285}
			b_{i}^{(T)}=0 .
		\end{equation}
		
		\noindent This system can alternatively be written in matrix-vector form as
		
		\begin{equation}
			\label{eqa286}
			\mu K c^{(w)}=0 b^{(w)}, \\
		\end{equation}

		\begin{equation}
			\label{eqa287}
			L c^{(w)}+\kappa K c^{(T)}=0
		\end{equation}
	
		\noindent with $L$ as the matrix from the $\nabla w_{-} \cdot \nabla$ operator: $L_{i, j}=A_{i, j}^{(w, T)}$.\smallbreak
		The matrix-vector equations are often conveniently written in block form:
		$$
		\left(\begin{array}{cc}
			\mu K & 0 \\
			L & \kappa K
		\end{array}\right)\left(\begin{array}{c}
			c^{(w)} \\
			c^{(T)}
		\end{array}\right)=\left(\begin{array}{c}
			b^{(w)} \\
			0
		\end{array}\right)
		$$\smallbreak
		Note that in the general case where all unknowns enter all equations, we have to solve the compound system (\ref{eqa297})-(\ref{eqa298}) since then we cannot utilize the special property that (\ref{eqa270}) does not involve $T$ and can be solved first.
		
		When the viscosity depends on the temperature, the $\mu \nabla^{2} w$ term must be replaced by $\nabla \cdot(\mu(T) \nabla w)$, and then $T$ enters the equation for $w$. Now we have a two-way coupling since both equations contain $w$ and $T$ and therefore must be solved simultaneously Th equation $\nabla \cdot(\mu(T) \nabla w)=-\beta$ is nonlinear, and if some iteration procedure is invoked, where we use a previously computed $T_{-}$in the viscosity $\left(\mu\left(T_{-}\right)\right)$, the coefficient is known, and the equation involves only one unknown, $w$. In that case we are back to the one-way coupled set of PDEs.
		
		We may also formulate our PDE system as a vector equation. To this end, we introduce the vector of unknowns $\boldsymbol{u}=\left(u^{(0)}, u^{(1)}\right)$, where $u^{(0)}=w$ and $u^{(1)}=T$. We then have
		$$
		\nabla^{2} u=\left(\begin{array}{c}
			-\mu^{-1} \beta \\
			-\kappa^{-1} \mu \nabla u^{(0)} \cdot \nabla u^{(0)}
		\end{array}\right)
		$$
	\section[Different function spaces for the unknowns]{Different function spaces for the unknowns}
		\label{sec:sec_20_4}
		\noindent It is easy to generalize the previous formulation to the case where $w \in V^{(w)}$ and $T \in V^{(T)}$, where $V^{(w)}$ and $V^{(T)}$ can be different spaces with different numbers of degrees of freedom. For example, we may use quadratic basis functions for $w$ and linear for $T$. Approximation of the unknowns by different finite element spaces is known as \emph{mixed finite} element methods.\smallbreak
		We write
		$$
		\begin{aligned}
			&V^{(w)}=\operatorname{span}\left\{\psi_{0}^{(w)}, \ldots, \psi_{N_{w}}^{(w)}\right\}, 
			&V^{(T)}=\operatorname{span}\left\{\psi_{0}^{(T)}, \ldots, \psi_{N_{T}}^{(T)}\right\} .
		\end{aligned}
		$$
		The next step is to multiply (\ref{eqa260}) by a test function $v^{(w)} \in V^{(w)}$ and (\ref{eqa261}) by a $v^{(T)} \in V^{(T)}$, integrate by parts and arrive at
		
		
		\begin{equation}
			\label{eqa288}
			\int_{\Omega} \mu \nabla w \cdot \nabla v^{(w)} \mathrm{d} x=\int_{\Omega} \beta v^{(w)} \mathrm{d} x \quad \forall v^{(w)} \in V^{(w)} \\
		\end{equation}
	
		\begin{equation}
			\label{eqa289}
			\int_{\Omega} \kappa \nabla T \cdot \nabla v^{(T)} \mathrm{d} x=\int_{\Omega} \mu \nabla w \cdot \nabla w v^{(T)} \mathrm{d} x \quad \forall v^{(T)} \in V^{(T)}
		\end{equation}
	
		The compound scalar variational formulation applies a test vector function $\boldsymbol{v}=\left(v^{(w)}, v^{(T)}\right)$ and reads
		
		\begin{equation}
			\label{eqa290}
			\int_{\Omega}\left(\mu \nabla w \cdot \nabla v^{(w)}+\kappa \nabla T \cdot \nabla v^{(T)}\right) \mathrm{d} x=\int_{\Omega}\left(\beta v^{(w)}+\mu \nabla w \cdot \nabla w v^{(T)}\right) \mathrm{d} x
		\end{equation}
		
		\noindent valid $\forall \boldsymbol{v} \in \boldsymbol{V}=V^{(w)} \times V^{(T)}$.\smallbreak
		The associated linear system is similar to (\ref{eqa270})-(\ref{eqa271}) or (\ref{eqa297})-(\ref{eqa298}), except that we need to distinguish between $\psi_{i}^{(w)}$ and $\psi_{i}^{(T)}$, and the range in the sums over $j$ must match the number of degrees of freedom in the spaces $V^{(w)}$ and $V^{(T)}$. The formulas become
		
		\begin{equation}
			\label{eqa291}
			\sum_{j=0}^{N_{w}} A_{i, j}^{(w)} c_{j}^{(w)}=b_{i}^{(w)}, \quad i=0, \ldots, N_{w}, \\
		\end{equation}
		
		\begin{equation}
			\label{eqa292}
			\sum_{j=0}^{N_{T}} A_{i, j}^{(T)} c_{j}^{(T)}=b_{i}^{(T)}, \quad i=0, \ldots, N_{T}, \\
		\end{equation}
	
		\begin{equation}
			\label{eqa293}
			A_{i, j}^{(w)}=\mu\left(\nabla \psi_{j}^{(w)}, \psi_{i}^{(w)}\right) \\
		\end{equation}
	
		\begin{equation}
			\label{eqa294}
			b_{i}^{(w)}=\left(\beta, \psi_{i}^{(w)}\right), \\
		\end{equation}
	
		\begin{equation}
			\label{eqa295}
			A_{i, j}^{(T)}=\kappa\left(\nabla \psi_{j}^{(T)}, \psi_{i}^{(T)}\right) \\
		\end{equation}
	
		\begin{equation}
			\label{eqa296}
			b_{i}^{(T)}=\mu\left(\nabla w_{-}, \psi_{i}^{(T)}\right)
		\end{equation}
		
		In the case we formulate one compound linear system involving both $c_{j}^{(w)}$, $j=0, \ldots, N_{w}$, and $c_{j}^{(T)}, j=0, \ldots, N_{T}$,(\ref{eqa297})-(\ref{eqa298}) becomes

		\begin{equation}
			\label{eqa297}
			\sum_{j=0}^{N_{w}} A_{i, j}^{(w, w)} c_{j}^{(w)}+\sum_{j=0}^{N_{T}} A_{i, j}^{(w, T)} c_{j}^{(T)}=b_{i}^{(w)}, \quad i=0, \ldots, N_{w} \\
		\end{equation}
	
		\begin{equation}
			\label{eqa298}
			\sum_{j=0}^{N_{w}} A_{i, j}^{(T, w)} c_{j}^{(w)}+\sum_{j=0}^{N_{T}} A_{i, j}^{(T, T)} c_{j}^{(T)}=b_{i}^{(T)}, \quad i=0, \ldots, N_{T}, \\
		\end{equation}
	
		\begin{equation}
			\label{eqa299}
			A_{i, j}^{(w, w)}=\mu\left(\nabla \psi_{j}^{(w)}, \psi_{i}^{(w)}\right) \\
		\end{equation}
		
		\begin{equation}
			\label{eqa300}
			A_{i, j}^{(w, T)}=0 \\
		\end{equation}
	
		\begin{equation}
			\label{eqa301}	
			b_{i}^{(w)}=\left(\beta, \psi_{i}^{(w)}\right), \\
		\end{equation}
		
		\begin{equation}
			\label{eqa302}	
			A_{i, j}^{(w, T)}\left.=\mu\left(\nabla w_{-} \cdot \nabla \psi_{j}^{(w)}\right), \psi_{i}^{(T)}\right) \\
		\end{equation}

		\begin{equation}
			\label{eqa303}
			A_{i, j}^{(T, T)}=\kappa\left(\nabla \psi_{j}^{(T)}, \psi_{i}^{(T)}\right) \\
		\end{equation}
	
		\begin{equation}
			\label{304}	
			b_{i}^{(T)}=0
		\end{equation}
		
		\noindent The corresponding block form
		$$
		\left(\begin{array}{cc}
			\mu K^{(w)} & 0 \\
			L & \kappa K^{(T)}
		\end{array}\right)\left(\begin{array}{c}
			c^{(w)} \\
			c^{(T)}
		\end{array}\right)=\left(\begin{array}{c}
			b^{(w)} \\
			0
		\end{array}\right)
		$$
		has square and rectangular block matrices: $K^{(w)}$ is $N_{w} \times N_{w}, K^{(T)}$ is $N_{T} \times N_{T}$, while $L$ is $N_{T} \times N_{w}$,
	\section[Computations in 1D]{Computations in 1D}
		\label{sec:sec_20_5}
		\noindent We can reduce the system (\ref{eqa260})-(\ref{eqa261}) to one space dimension, which corresponds to flow in a channel between two flat plates. Alternatively, one may consider flow in a circular pipe, introduce cylindrical coordinates, and utilize the radial symmetry to reduce the equations to a one-dimensional problem in the radial coordinate. The former model becomes
		
		\begin{equation}
			\label{eqa305}
			\mu w_{x x}=-\beta, \\
		\end{equation}
	
		\begin{equation}
		\label{eqa306}
			kappa T_{x x}=-\mu w_{x}^{2},
		\end{equation}
		
		\noindent while the model in the radial coordinate $r$ reads
		
		\begin{equation}
			\label{eqa307}
			\mu \frac{1}{r} \frac{d}{d r}\left(r \frac{d w}{d r}\right)=-\beta \\
		\end{equation}
		
		\begin{equation}
			\label{eqa308}
			\kappa \frac{1}{r} \frac{d}{d r}\left(r \frac{d T}{d r}\right)=-\mu\left(\frac{d w}{d r}\right)^{2}
		\end{equation}
		
		The domain for (\ref{eqa305}) - (\ref{eqa306}) is $\Omega=[0, H]$, with boundary conditions $w(0)=$ $w(H)=0$ and $T(0)=T(H)=T_{0}$. For (\ref{eqa307})-(\ref{eqa308}) the domain is $[0, R]$ ( $R$ being the radius of the pipe) and the boundary conditions are $d u / d r=d T / d r=0$ for $r=0, u(R)=0$, and $T(R)=T_{0} .$\smallbreak
		\textbf{Calculations to be continued...}
	


\clearpage
\end{document} 
